trillium/program_logic/simulation_adequacy_em.v
@@ -11,7 +11,8 @@ Section adequacy.
   
   Definition wp_premise
     (Σ: gFunctors)
-    (s: stuckness) (e: expr Λ) σ1 (s1: mstate M)
+    (s: stuckness) (f: forks_bit)
+    (e: expr Λ) σ1 (s1: mstate M)
     (p: em_init_param)
     := 
     (∀ `{Hinv : @IEMGS _ _ LG_EM EM Σ},
@@ -21,12 +22,13 @@ Section adequacy.
              em_init_resource s1 p (em_GS0 := iem_fairnessGS _ _)
            ={⊤}=∗
               config_wp ∗
-              WP e @ s; locale_of [] e; ⊤ {{ v, em_thread_post (locale_of [] e) v (em_GS0 := eGS) }} ∗
+              WP e @ f; s; locale_of [] e; ⊤ {{ v, em_thread_post (locale_of [] e) v (em_GS0 := eGS) }} ∗
               rel_always_holds0 R s state_interp (fun v => em_thread_post (locale_of [] e) v (em_GS0 := eGS)) e σ1 s1)).
 
   Definition wp_premise_multiple
     (Σ: gFunctors)
-    (s: stuckness) es σ1 (s1: mstate M)
+    (s: stuckness) f 
+    es σ1 (s1: mstate M)
     (p: em_init_param)
     := 
     (∀ `{Hinv : @IEMGS _ _ LG_EM EM Σ},
@@ -36,12 +38,12 @@ Section adequacy.
            ={⊤}=∗
               let Φs := map (fun τ v => em_thread_post τ v (em_GS0 := iem_fairnessGS _ _)) (locales_of_list es) in
               config_wp ∗
-              wptp s es Φs ∗
+              wptp s f es Φs ∗
               rel_always_holds s Φs R (es, σ1) s1)).
 
   Lemma wp_premise_single Σ
-    s (e1: expr Λ) σ1 s1 p:
-    wp_premise Σ s e1 σ1 s1 p -> wp_premise_multiple Σ s [e1] σ1 s1 p.
+    s f (e1: expr Λ) σ1 s1 p:
+    wp_premise Σ s f e1 σ1 s1 p -> wp_premise_multiple Σ s f [e1] σ1 s1 p.
   Proof using.
     rewrite /wp_premise /wp_premise_multiple.
     iIntros "%WP1 % [HEAP INIT]".
@@ -51,18 +53,19 @@ Section adequacy.
 
   Theorem strong_simulation_adequacy_general_multiple
     `{hPre: @IEMGpreS _ _ LG_EM EM Σ}
-    (s: stuckness) es σ1 (s1: M)
+    (s: stuckness) f 
+    es σ1 (s1: M)
     (p: em_init_param)    
     :
     length es ≥ 1 ->
     rel_finitary R →
     em_is_init_st (es, σ1) s1 ->
     em_valid_state_evolution_fairness {tr[ (es, σ1) ]} {tr[ s1 ]} ->
-    (wp_premise_multiple Σ s es σ1 s1 p) ->
+    (wp_premise_multiple Σ s f es σ1 s1 p) ->
     continued_simulation R (trace_singleton (es, σ1)) (trace_singleton s1).
   Proof.
     intros LEN Hfin INIT VALID1 WPS.
-    apply (wp_strong_adequacy_multiple_with_trace_inv Λ M Σ s); try done.
+    apply (wp_strong_adequacy_multiple_with_trace_inv Λ M Σ s f); try done.
 
     iIntros (?) "".
 
@@ -93,7 +96,7 @@ Section adequacy.
   Qed.
 
   Theorem strong_simulation_adequacy_inftraces_multiple Σ
-    `{hPre: @IEMGpreS _ _ LG_EM EM Σ} (s: stuckness) 
+    `{hPre: @IEMGpreS _ _ LG_EM EM Σ} (s: stuckness) f
     es σ1 (s1: M)
     (p: em_init_param)
     (iex : inf_execution_trace Λ)
@@ -102,7 +105,7 @@ Section adequacy.
     length es ≥ 1 ->
     rel_finitary R →
     em_is_init_st (es, σ1) s1 ->
-    (wp_premise_multiple Σ s es σ1 s1 p) ->
+    (wp_premise_multiple Σ s f es σ1 s1 p) ->
     exists iatr,
       @valid_inf_system_trace _ M
         (@continued_simulation Λ M R)
@@ -121,7 +124,7 @@ Section adequacy.
   Qed.
   
   Theorem strong_simulation_adequacy_traces_multiple Σ
-    `{hPre: @IEMGpreS _ _ LG_EM EM Σ} (s: stuckness) 
+    `{hPre: @IEMGpreS _ _ LG_EM EM Σ} (s: stuckness) f
     es σ1 (s1: M)
     (p: em_init_param)
     extr
@@ -145,7 +148,7 @@ Section adequacy.
     length es ≥ 1 ->
     rel_finitary R →
     em_is_init_st (es, σ1) s1 ->
-    (wp_premise_multiple Σ s es σ1 s1 p) ->
+    (wp_premise_multiple Σ s f es σ1 s1 p) ->
     ∃ (mtr : trace (mstate M) (mlabel M)), 
       traces_match lbl_rel state_rel locale_step (@mtrans M) extr mtr /\
       trfirst mtr = s1. 
@@ -192,7 +195,7 @@ Section adequacy.
   Qed.
   
   Theorem strong_simulation_adequacy_traces Σ
-    `{hPre: @IEMGpreS _ _ LG_EM EM Σ} (s: stuckness) 
+    `{hPre: @IEMGpreS _ _ LG_EM EM Σ} (s: stuckness) f
     (e: expr Λ) σ1 (s1: M)
     (p: em_init_param)
     extr
@@ -215,7 +218,7 @@ Section adequacy.
     :
     rel_finitary R →
     em_is_init_st ([e], σ1) s1 ->
-    (wp_premise Σ s e σ1 s1 p) ->
+    (wp_premise Σ s f e σ1 s1 p) ->
     ∃ (mtr : trace (mstate M) (mlabel M)), 
       traces_match lbl_rel state_rel locale_step (@mtrans M) extr mtr /\
       trfirst mtr = s1. 
