trillium/program_logic/ectx_lifting.v
@@ -7,6 +7,7 @@ Set Default Proof Using "Type".
 Section wp.
 Context {Λ : ectxLanguage} `{!irisG Λ M Σ} {Hinh : Inhabited (state Λ)}.
 Implicit Types s : stuckness.
+Implicit Types f : forks_bit.
 Implicit Types P : iProp Σ.
 Implicit Types Φ : val Λ → iProp Σ.
 Implicit Types v : val Λ.
@@ -17,7 +18,7 @@ Local Definition reducible_not_val_inhabitant e :=
 Hint Resolve reducible_not_val_inhabitant : core.
 Hint Resolve head_stuck_stuck : core.
 
-Lemma wp_lift_head_step_fupd {s E Φ} e1 ζ:
+Lemma wp_lift_head_step_fupd {s f E Φ} e1 ζ:
   to_val e1 = None →
   (∀ (extr : execution_trace Λ) (atr : auxiliary_trace M) K tp1 tp2 σ1,
     ⌜valid_exec extr⌝ -∗
@@ -30,10 +31,11 @@ Lemma wp_lift_head_step_fupd {s E Φ} e1 ζ:
         state_interp
           (trace_extend extr (Some ζ) (tp1 ++ fill K e2 :: tp2 ++ efs, σ2))
           (trace_extend atr ℓ δ2) ∗
-      WP e2 @ s; ζ; E {{ Φ }} ∗
-      [∗ list] i ↦ef ∈ efs, WP ef @ s; locale_of (tp1 ++ ectx_fill K e1 :: tp2 ++ (take i efs)) ef; ⊤
-         {{ fork_post (locale_of (tp1 ++ ectx_fill K e1 :: tp2 ++ (take i efs)) ef) }})
-  ⊢ WP e1 @ s; ζ; E {{ Φ }}.
+      WP e2 @ f; s; ζ; E {{ Φ }} ∗
+      ([∗ list] i ↦ef ∈ efs, WP ef @ f; s; locale_of (tp1 ++ ectx_fill K e1 :: tp2 ++ (take i efs)) ef; ⊤
+         {{ fork_post (locale_of (tp1 ++ ectx_fill K e1 :: tp2 ++ (take i efs)) ef) }}) ∗ 
+      ⌜ f = CannotFork -> efs = [] ⌝ )
+  ⊢ WP e1 @ f; s; ζ; E {{ Φ }}.
 Proof.
   iIntros (?) "H". iApply wp_lift_step_fupd=>//.
   iIntros (ex atr K tp1 tp2 σ1 Hexvalid hex Hloc) "Hsi".
@@ -41,10 +43,10 @@ Proof.
   iModIntro.
   iSplit; first by destruct s; eauto.
   iIntros (e2 σ2 efs ?).
-  iApply "H"; eauto.
+  iApply "H"; eauto.  
 Qed.
 
-Lemma wp_lift_head_step {s E Φ} e1 ζ:
+Lemma wp_lift_head_step {s f E Φ} e1 ζ:
   to_val e1 = None →
   (∀ (extr : execution_trace Λ) (atr : auxiliary_trace M) K tp1 tp2 σ1,
     ⌜valid_exec extr⌝ -∗
@@ -56,10 +58,11 @@ Lemma wp_lift_head_step {s E Φ} e1 ζ:
         state_interp
           (trace_extend extr (Some ζ) (tp1 ++ fill K e2 :: tp2 ++ efs, σ2))
           (trace_extend atr ℓ δ2) ∗
-      WP e2 @ s; ζ; E {{ Φ }} ∗
-      [∗ list] i ↦ef ∈ efs, WP ef @ s; locale_of (tp1 ++ ectx_fill K e1 :: tp2 ++ (take i efs)) ef; ⊤
-         {{ fork_post (locale_of (tp1 ++ ectx_fill K e1 :: tp2 ++ (take i efs)) ef) }})
-  ⊢ WP e1 @ s; ζ; E {{ Φ }}.
+      WP e2 @ f; s; ζ; E {{ Φ }} ∗
+      ([∗ list] i ↦ef ∈ efs, WP ef @ f; s; locale_of (tp1 ++ ectx_fill K e1 :: tp2 ++ (take i efs)) ef; ⊤
+         {{ fork_post (locale_of (tp1 ++ ectx_fill K e1 :: tp2 ++ (take i efs)) ef) }}) ∗ 
+    ⌜ f = CannotFork -> efs = [] ⌝)
+  ⊢ WP e1 @ f; s; ζ; E {{ Φ }}.
 Proof.
   iIntros (?) "H". iApply wp_lift_head_step_fupd; [done|]. iIntros (?????????) "?".
   iMod ("H" with "[//] [//] [$]") as "[$ H]".
@@ -67,31 +70,31 @@ Proof.
   iApply "H"; done.
 Qed.
 
-Lemma wp_lift_head_stuck E Φ e ζ:
+Lemma wp_lift_head_stuck f E Φ e ζ:
   to_val e = None →
   sub_redexes_are_values e →
   (∀ (extr : execution_trace Λ) (atr : auxiliary_trace M) K tp1 tp2 σ,
     ⌜valid_exec extr⌝ -∗
     ⌜trace_ends_in extr (tp1 ++ fill K e :: tp2, σ)⌝ →
     state_interp extr atr ={E,∅}=∗ ⌜head_stuck e σ⌝)
-  ⊢ WP e @ ζ; E ?{{ Φ }}.
+  ⊢ WP e @ f; MaybeStuck; ζ; E {{ Φ }}.
 Proof.
   iIntros (??) "H". iApply wp_lift_stuck; first done.
   iIntros (????????) "Hsi". iMod ("H" with "[] [] Hsi") as "%"; by auto.
 Qed.
 
-Lemma wp_lift_pure_head_stuck E Φ e :
+Lemma wp_lift_pure_head_stuck f ζ E Φ e :
   to_val e = None →
   sub_redexes_are_values e →
   (∀ σ, head_stuck e σ) →
-  ⊢ WP e @ E ?{{ Φ }}.
+  ⊢ WP e @ f; MaybeStuck; ζ; E {{ Φ }}.
 Proof using Hinh.
   iIntros (?? Hstuck). iApply wp_lift_head_stuck; [done|done|].
   iIntros (???????) "_". iMod (fupd_mask_subseteq ∅) as "_"; first set_solver.
   auto; done.
 Qed.
 
-Lemma wp_lift_atomic_head_step_fupd {s E1 E2 Φ} e1 ζ:
+Lemma wp_lift_atomic_head_step_fupd {s f E1 E2 Φ} e1 ζ:
   to_val e1 = None →
   (∀ (extr : execution_trace Λ) (atr : auxiliary_trace M) K tp1 tp2 σ1,
     ⌜valid_exec extr⌝ -∗
@@ -105,9 +108,9 @@ Lemma wp_lift_atomic_head_step_fupd {s E1 E2 Φ} e1 ζ:
           (trace_extend extr (Some ζ) (tp1 ++ fill K e2 :: tp2 ++ efs, σ2))
           (trace_extend atr ℓ δ2) ∗
       from_option Φ False (to_val e2) ∗
-      [∗ list] i ↦ef ∈ efs, WP ef @ s; locale_of (tp1 ++ ectx_fill K e1 :: tp2 ++ (take i efs)) ef; ⊤
-         {{ fork_post (locale_of (tp1 ++ ectx_fill K e1 :: tp2 ++ (take i efs)) ef) }})
-  ⊢ WP e1 @ s; ζ; E1 {{ Φ }}.
+      ([∗ list] i ↦ef ∈ efs, WP ef @ f; s; locale_of (tp1 ++ ectx_fill K e1 :: tp2 ++ (take i efs)) ef; ⊤
+         {{ fork_post (locale_of (tp1 ++ ectx_fill K e1 :: tp2 ++ (take i efs)) ef) }}) ∗ ⌜ f = CannotFork -> efs = [] ⌝)
+  ⊢ WP e1 @ f; s; ζ; E1 {{ Φ }}.
 Proof.
   iIntros (?) "H". iApply wp_lift_atomic_step_fupd; [done|].
   iIntros (?????????) "Hsi". iMod ("H" with "[//] [//] [//] Hsi") as "[% H]".
@@ -117,7 +120,7 @@ Proof.
   iApply "H"; eauto.
 Qed.
 
-Lemma wp_lift_atomic_head_step {s E Φ} e1 ζ:
+Lemma wp_lift_atomic_head_step {s f E Φ} e1 ζ:
   to_val e1 = None →
   (∀ (extr : execution_trace Λ) (atr : auxiliary_trace M) K tp1 tp2 σ1,
     ⌜valid_exec extr⌝ -∗
@@ -131,9 +134,10 @@ Lemma wp_lift_atomic_head_step {s E Φ} e1 ζ:
           (trace_extend extr (Some ζ) (tp1 ++ fill K e2 :: tp2 ++ efs, σ2))
           (trace_extend atr ℓ δ2) ∗
       from_option Φ False (to_val e2) ∗
-      [∗ list] i ↦ef ∈ efs, WP ef @ s; locale_of (tp1 ++ ectx_fill K e1 :: tp2 ++ (take i efs)) ef; ⊤
-         {{ fork_post (locale_of (tp1 ++ ectx_fill K e1 :: tp2 ++ (take i efs)) ef) }})
-  ⊢ WP e1 @ s; ζ; E {{ Φ }}.
+      ([∗ list] i ↦ef ∈ efs, WP ef @ f; s; locale_of (tp1 ++ ectx_fill K e1 :: tp2 ++ (take i efs)) ef; ⊤
+         {{ fork_post (locale_of (tp1 ++ ectx_fill K e1 :: tp2 ++ (take i efs)) ef) }}) ∗
+    ⌜ f = CannotFork -> efs = [] ⌝)
+  ⊢ WP e1 @ f; s; ζ; E {{ Φ }}.
 Proof.
   iIntros (?) "H". iApply wp_lift_atomic_step; eauto.
   iIntros (?????????) "Hsi". iMod ("H" with "[//] [//] [//] Hsi") as "[% H]".
@@ -142,7 +146,7 @@ Proof.
   iApply "H"; eauto.
 Qed.
 
-Lemma wp_lift_atomic_head_step_no_fork_fupd {s E1 E2 Φ} e1 ζ:
+Lemma wp_lift_atomic_head_step_no_fork_fupd {s f E1 E2 Φ} e1 ζ:
   to_val e1 = None →
   (∀ (extr : execution_trace Λ) (atr : auxiliary_trace M) K tp1 tp2 σ1,
     ⌜valid_exec extr⌝ -∗
@@ -157,7 +161,7 @@ Lemma wp_lift_atomic_head_step_no_fork_fupd {s E1 E2 Φ} e1 ζ:
           (trace_extend extr (Some ζ) (tp1 ++ fill K e2 :: tp2 ++ efs, σ2))
           (trace_extend atr ℓ δ2) ∗
       from_option Φ False (to_val e2))
-  ⊢ WP e1 @ s; ζ; E1 {{ Φ }}.
+  ⊢ WP e1 @ f; s; ζ; E1 {{ Φ }}.
 Proof.
   iIntros (?) "H". iApply wp_lift_atomic_head_step_fupd; [done|].
   iIntros (?????????) "Hsi".
@@ -167,10 +171,10 @@ Proof.
   iMod ("H" $! v2 σ2 efs with "[# //]") as "H".
   iIntros "!> !>". iMod "H" as (st' ℓ) "(-> & ? & ?) /=".
   iModIntro; iExists _, _.
-  iFrame.
+  by iFrame. 
 Qed.
 
-Lemma wp_lift_atomic_head_step_no_fork {s E Φ} e1 ζ:
+Lemma wp_lift_atomic_head_step_no_fork {s f E Φ} e1 ζ:
   to_val e1 = None →
   (∀ (extr : execution_trace Λ) (atr : auxiliary_trace M) K tp1 tp2 σ1,
     ⌜valid_exec extr⌝ -∗
@@ -184,7 +188,7 @@ Lemma wp_lift_atomic_head_step_no_fork {s E Φ} e1 ζ:
           (trace_extend extr (Some ζ) (tp1 ++ fill K e2 :: tp2 ++ efs, σ2))
           (trace_extend atr ℓ δ2) ∗
       from_option Φ False (to_val e2))
-  ⊢ WP e1 @ s; ζ; E {{ Φ }}.
+  ⊢ WP e1 @ f; s; ζ; E {{ Φ }}.
 Proof.
   iIntros (?) "H". iApply wp_lift_atomic_head_step; eauto.
   iIntros (?????????) "Hsi".
@@ -193,30 +197,30 @@ Proof.
   iNext; iIntros (v2 σ2 efs Hstep).
   iMod ("H" $! v2 σ2 efs with "[//]") as (st' ℓ) "(-> & ? & ?) /=".
   iModIntro; iExists _, _.
-  iFrame.
+  by iFrame.
 Qed.
 
 Lemma wp_lift_pure_det_head_step_no_fork
-      `{!AllowsPureStep M Σ}  {s E E' Φ} e1 e2 ζ:
+      `{!AllowsPureStep M Σ}  {s f E E' Φ} e1 e2 ζ:
   to_val e1 = None →
   (∀ σ1, head_reducible e1 σ1) →
   (∀ σ1 e2' σ2 efs',
     head_step e1 σ1 e2' σ2 efs' → σ2 = σ1 ∧ e2' = e2 ∧ efs' = []) →
-  (|={E}[E']▷=> WP e2 @ s; ζ; E {{ Φ }}) ⊢ WP e1 @ s; ζ; E {{ Φ }}.
+  (|={E}[E']▷=> WP e2 @ f; s; ζ; E {{ Φ }}) ⊢ WP e1 @ f; s; ζ; E {{ Φ }}.
 Proof using Hinh.
   intros. rewrite -(wp_lift_pure_det_step_no_fork e1 e2); eauto.
   destruct s; by auto.
 Qed.
 
 Lemma wp_lift_pure_det_head_step_no_fork'
-      `{!AllowsPureStep M Σ} {s E Φ} e1 e2 ζ:
+      `{!AllowsPureStep M Σ} {s f E Φ} e1 e2 ζ:
   to_val e1 = None →
   (∀ σ1, head_reducible e1 σ1) →
   (∀ σ1 e2' σ2 efs',
     head_step e1 σ1 e2' σ2 efs' → σ2 = σ1 ∧ e2' = e2 ∧ efs' = []) →
-  ▷ WP e2 @ s; ζ; E {{ Φ }} ⊢ WP e1 @ s; ζ; E {{ Φ }}.
+  ▷ WP e2 @ f; s; ζ; E {{ Φ }} ⊢ WP e1 @ f; s; ζ; E {{ Φ }}.
 Proof using Hinh.
-  intros. rewrite -[(WP e1 @ s; _; _ {{ _ }})%I]wp_lift_pure_det_head_step_no_fork //.
+  intros. rewrite -[(WP e1 @ f; s; _; _ {{ _ }})%I]wp_lift_pure_det_head_step_no_fork //.
   rewrite -step_fupd_intro //.
 Qed.
 End wp.
